proved the necessary lemma

PoS/Semantics.v
@@ -16,8 +16,55 @@ Parameter N : nat.
 Definition PacketSoup := seq Packet.
 
 Definition StateMap := union_map [ordType of nid] State.
-Definition initState : StateMap :=
-foldr (PCM.join) (0 \\-> Init 0) (map (fun i => i \\-> Init i) (iota 1 N)).
+
+Fixpoint initState' n : StateMap :=
+  if n is n'.+1 then (n \\-> Init n) \+ (initState' n') else Unit.
+
+(* Master-lemma, proving a conjunction of two mutually-necessary facts *)
+Lemma initStateValidDom n : dom (initState' n) =i iota 1 n /\ valid (initState' n).
+Proof.
+elim: n=>/=[|n [H1 H2]]; first by rewrite valid_unit dom0.
+split; last first.
+- case: validUn; rewrite ?um_validPt ?H2//. 
+  move=>k; rewrite um_domPt inE=>/eqP Z; subst k.
+  by rewrite H1 mem_iota=>/andP[_]; rewrite add1n ltnn. 
+move=>z; rewrite domUn !inE !um_domPt !inE.
+case B: (z == 1)=>//=.
+- move/eqP: B=>B; subst z=>/=; apply/andP; split; last first.
+  + by rewrite orbC H1 mem_iota/= addnC addn1; case: n {H1 H2}=>//.
+  case: validUn; rewrite ?um_validPt ?H2//. 
+  move=>k; rewrite um_domPt inE=>/eqP Z; subst k.
+  by rewrite H1 mem_iota=>/andP[_]; rewrite add1n ltnn. 
+case C: (z \in iota 2 n).
+- apply/andP; split; last first.
+  + rewrite orbC H1 mem_iota/= addnC addn1; rewrite mem_iota in C.
+    case/andP: C=>H3 H4; rewrite eq_sym.
+    rewrite addnC addn2 in H4; clear B.
+    case B: (z == n.+1); rewrite orbC//=.
+    rewrite ltnS leq_eqVlt B/= in H4.
+    by rewrite H4 andbC/=; by case: {B H4} z H3.
+  case: validUn; rewrite ?um_validPt ?H2//. 
+  move=>k; rewrite um_domPt inE=>/eqP Z; subst k. 
+  by rewrite H1 mem_iota=>/andP[_]; rewrite add1n ltnn. 
+rewrite H1; apply/negP=>/andP[_]/orP[].
+- move/eqP=>Z; subst z; rewrite mem_iota in C.
+  move/negP: C=>C; apply: C; rewrite addnC addn2.
+  rewrite andbC ltnSn/=; clear H1 H2.
+  by move/negbT: B; case: n.
+rewrite !mem_iota in C *=>/andP[]H3 H4.
+move/negP: C=>C; apply: C; apply/andP; split.
+- by clear H4; case: z H3 B=>//z _; case: z=>//.
+rewrite addnC addn1 in H4; rewrite addnC.
+by rewrite addn2 -[n.+2]addn1; apply: ltn_addr. 
+Qed.
+
+Lemma valid_initState n : valid (initState' n).
+Proof. by case: (initStateValidDom n). Qed.
+
+Lemma dom_initState n : dom (initState' n) =i iota 1 n.
+Proof. by case: (initStateValidDom n). Qed.
+
+Definition initState := initState' N.
 
 Record World :=
   mkW {
@@ -69,8 +116,29 @@ Definition Coh (w : World) :=
 
 Lemma Coh_init : Coh initWorld.
 Proof.
-rewrite /Coh /holds. move=> n st.
-move=> fW. specialize (find_some fW)=> dW.
-rewrite /initWorld /initState /localState in dW.
-Search "um_findPt_inv".
-Admitted.
+move=>n st.
+rewrite /initWorld/initState/localState/=.
+(* Since the state is constructed inductively, use induction on N *)
+elim: N=>//=[|n' Hi].
+  (* Using facts about union-maps. *)
+- Search _ (find) (Some).
+  move/find_some.
+  (* Domain of an empty map should be empty, right? *)
+  Search _ (dom _) (Unit).
+  rewrite dom0.
+  (* Fiddling with \in predicate *)
+  rewrite inE.
+  done.
+
+(* The main induction transition. *)
+(* Can we doe somthingabout find of a union? *)
+Search _ (find) (_ \+ _).
+rewrite findUnL; last first.
+- case: validUn; rewrite ?um_validPt ?valid_initState//.
+  move=>k; rewrite um_domPt !inE=>/eqP Z; subst k.
+  by rewrite dom_initState mem_iota addnC addn1 ltnn andbC. 
+case: ifP=>//D.
+rewrite um_domPt inE in D; move/eqP:D=>D; subst n.
+by rewrite um_findPt; case=><-.  
+Qed.  
+  
